cequiv/extensional_ldepth.v
@@ -1,0 +1,50 @@
+(*
+
+  Copyright 2014 Cornell University
+  Copyright 2015 Cornell University
+  Copyright 2016 Cornell University
+  Copyright 2017 Cornell University
+  Copyright 2018 Cornell University
+
+  This file is part of VPrl (the Verified Nuprl project).
+
+  VPrl is free software: you can redistribute it and/or modify
+  it under the terms of the GNU General Public License as published by
+  the Free Software Foundation, either version 3 of the License, or
+  (at your option) any later version.
+
+  VPrl is distributed in the hope that it will be useful,
+  but WITHOUT ANY WARRANTY; without even the implied warranty of
+  MERCHANTABILITY or FITNESS FOR A PARTICULAR PURPOSE.  See the
+  GNU General Public License for more details.
+
+  You should have received a copy of the GNU General Public License
+  along with VPrl.  If not, see <http://www.gnu.org/licenses/>.
+
+
+  Websites: http://nuprl.org/html/verification/
+            http://nuprl.org/html/Nuprl2Coq
+            https://github.com/vrahli/NuprlInCoq
+
+  Authors: Abhishek Anand & Vincent Rahli
+
+*)
+
+
+Require Import approx_star0.
+
+
+Lemma extensional_ldepth {p} : extensional_op (@NCan p NLDepth).
+Proof.
+  introv Hpra Hprt Hprt' Hcv Has Hi.
+
+  applydup @isprogram_ldepth_implies in Hprt; exrepnd; subst; cpx.
+  applydup @isprogram_ldepth_implies in Hprt'; exrepnd; subst; cpx.
+
+  apply computes_to_val_like_in_max_k_steps_S in Hcv; exrepnd.
+  csunf Hcv1; simpl in *; ginv.
+  apply computes_to_val_like_in_max_k_steps_if_isvalue_like in Hcv0; eauto 2 with slow; subst.
+  eapply approx_star_open_trans;
+    [|apply reduces_to_implies_approx_open1;[|apply reduces_to_if_step;csunf;simpl;auto] ];
+    eauto 2 with slow.
+Qed.
